
\section{Libor Market Model}


We suppose  $t \leq T_0 < T_1 <..<T_M $ with  $T_i=T_0+i \tau$ and  $T_{i+1}-T_i=\tau $ 
 

Recall that 

\ban
1+\tau L(t,T_i,\tau)=\frac{B(t,T_i)}{B(t,T_{i+1})} 
\ean

and

\ban
S(t,T_s,T_M)=\frac{B(t,T_s)-B(t,T_M)}{\sum_{j=s+1}^{M}\tau B(t,T_j)}
\ean

\ban
\frac{B(t,T_i)}{B(t,T_s)}=\prod_{j=s}^{i-1}\frac{1}{1+\tau L(t,T_j,\tau)}
\ean

as such the forward swap rate as a function of the forward rates is given by the relation

\ba
S(t,T_s,T_M)=\frac{1 - \prod_{j=s}^{M-1}\frac{1}{1+\tau L(t,T_j,\tau)} }{\sum_{j=s+1}^{M}\tau \prod_{k=s}^{j-1}\frac{1}{1+\tau L(t,T_k,\tau)}} \label{tswaptfor}
\ea

In the libor market model we suppose the following dynamic for the forward Libor rates


\ban
dL(t,T_i,\tau)=L(t,T_i,\tau)\gamma(t,T_i,\tau)dW^{Q^{T_{i+1}}}
\ean

where $\lbrace W^{Q^{T_{i+1}}}_t; t\geq 0 \rbrace$ is a $d$ dimensional brownian motion under the forward probability $Q^{T_{i+1}}$ associated with the numeraire $B(t,T_{i+1})$ and  $\gamma(t,T_i,\tau)$ is a deterministic function. 

Furthermore we know that 

\ban
d\left(\frac{B(t,T_i)}{B(t,T_{i+1})}\right)=\left( \frac{B(t,T_i)}{B(t,T_{i+1})} \right) (\sigma_B(t,T_i)-\sigma_B(t,T_{i+1}))dW^{Q^{T_{i+1}}}_t
\ean

where $\sigma_B(t,T)$ stands for the volatility of the zero coupon bond so from 

\ban
\frac{dL(t,T_i,\tau)}{L(t,T_i,\tau)}=\frac{1+\tau L(t,T_i,\tau)}{\tau L(t,T_i,\tau)}(\sigma_B(t,T_i)-\sigma_B(t,T_{i+1}))dW^{Q^{T_{i+1}}}_t
\ean

we get the relation

\ba
\frac{\gamma(t,T_i,\tau)\tau L(t,T_i,\tau)}{1+\tau L(t,T_i,\tau)}=\sigma_B(t,T_i)-\sigma_B(t,T_{i+1}) \label{volforvolzc}
\ea


this equation leads  from  (\ref{volforvolzc}) we have for  $j>i$

\ban
\sigma_B(t,T_j)-\sigma_B(t,T_i)=-\sum_{k=i}^{j-1}\frac{\gamma(t,T_k,\tau)\tau L(t,T_k,\tau)}{1+\tau L(t,T_k,\tau)}
\ean

it is well known that 

\ban
dW_t^{Q^{T_i}}+\sigma_B(t,T_i)dt=dW_t^{Q^{T_j}}+\sigma_B(t,T_j)dt
\ean

changing from zero coupon bond volatilities to forward rate volatilities we have for  $j>i$

\ban
dW_t^{Q^{T_i}}=dW_t^{Q^{T_j}}-\sum_{k=i}^{j-1}\frac{\gamma(t,T_k,\tau)\tau L(t,T_k,\tau)}{1+\tau L(t,T_k,\tau)}dt
\ean

\subsection{Pricing a caplet in the LMM framework}


Within the LMM the forward libor rate $L(t,T_i,\tau)$ follows the dynamic 

\ban
dL(t,T_i,\tau)=L(t,T_i,\tau)\gamma(t,T_i,\tau)dW^{Q^{T_{i+1}}}_t
\ean


suppose   $t<T_j<T_{j+1}$ and  $Cplt(t,T_j,K,\tau,N)$ a european  caplet with  maturity $T_j$,  strike $K$, nominal $N$  on the spot libor rate $L(t,t,\tau)$ then at time $T_{j+1}=T_j+\tau$ the cash flow is 

\ban
\tau (L(T_j,T_j,\tau)-K)_+N
\ean


\ban
Cplt(t,T_j,K,\tau,N)&=&E^Q_t\left[\frac{B(t)}{B(T_{j+1})}\tau (L(T_j,T_j,\tau)-K)_+N \right]\\
&=&E^{Q^{T_{j+1}}}_t\left[\frac{B(t,T_{j+1})}{B(T_{j+1},T_{j+1})}\tau (L(T_j,T_j,\tau)-K)_+N \right]\\
&=&B(t,T_{j+1}) N\tau E^{Q^{T_{j+1}}}_t\left[(L(T_j,T_j,\tau)-K)_+ \right]\\
&=& N \tau B(t,T_{j+1}) \left( L(t,T_{j},\tau)N(d_1)-KN(d_2)\right)
\ean

\ban
d_1&=&\frac{ln \frac{L(t,T_j,\tau)}{K} + \frac{1}{2}\int_t^{T_j}\gamma(u,T_j,\tau)^2du}{\sqrt{\int_t^{T_j}\gamma(u,T_j,\tau)^2 du}}\\
d_2&=&d_1 -\sqrt{\int_t^{T_j}\gamma(u,T_j,\tau)^2 du}
\ean


we get a formula consistent with market practice which quotes option through black volatility

\subsection{Pricing a swaption in the LMM framework}\label{DerPrdcts}

We briefly present the pricing of a swaption within the LMM framework and refer to \cite{braceGatarekMusiela}. Recall that 

\ban
Swpt(t,T_s,T_M,K,\tau)&=&\sum_{i=s+1}^ME^Q_t\left[ \frac{B(t)}{B(T_i)}\tau (S(T_s,T_s,T_M)-K)_+ \right]\\
&=&\tau \sum_{i=s+1}^MB(t,T_i)E^{Q^{T_i}}_t\left[L(T_s,T_{i-1},\tau){\bf 1}_{D}\right] \\
&-&\tau \sum_{i=s+1}^MB(t,T_i)E^{Q^{T_i}}_t\left[K{\bf 1}_{D}\right]
\ean

where

\ban
{\bf 1}_{D}&=&{\bf 1}_{\left( S(T_s,T_s,T_M)>K \right)}\\
&=&{\bf 1}_{\left( 1>B(T_s,T_M)+K\sum_{i=s+1}^MB(T_s,T_i)\right) }\\
&=&{\bf 1}_{\left( 1>\sum_{i=s+1}^Mc_iB(T_s,T_i)\right) }\\
&=&{\bf 1}_{\left( 1>\sum_{j=s+1}^Mc_j\prod_{k=0}^{j-1}\frac{1}{1+\tau L(T_s,T_j,\tau)} \right) } 
\ean


under  $Q^{T_i}$ we have  

\ban
dL(t,T_{i-1},\tau)=L(t,T_{i-1},\tau)\gamma(t,T_{i-1},\tau)dW^{Q^{T_{i}}}_t
\ean

for  $i>j+1$ 

\ban
\frac{dL(t,T_j,\tau)}{L(t,T_j,\tau)}=\gamma(t,T_j,\tau)dW^{Q^{T_i}}_t - \sum_{k=j+1}^{i-1}\frac{\tau L(t,T_k,\tau) \gamma(t,T_k,\tau) \gamma(t,T_j,\tau) }{1+\tau L(t,T_k,\tau)}dt
\ean

for  $j\geq i$ 

\ban
\frac{dL(t,T_j,\tau)}{L(t,T_j,\tau)}=\gamma(t,T_j,\tau)dW^{Q^{T_i}}_t +\sum_{k=i}^{j}\frac{\tau L(t,T_k,\tau)\gamma(t,T_k,\tau)\gamma(t,T_j,\tau)}{1+\tau L(t,T_k,\tau)}dt
\ean
 
\paragraph{Computing  $E^{Q^{T_i}}_t\left[L(T_s,T_{i-1},\tau){\bf 1}_{D}\right]$: }


Brace, Gatarek and Musiela  \cite{braceGatarekMusiela} propose to freeze the drift: under  $Q^{T_i}$ for  $i>j+1$ and $u \in [t \; T_s]$

\ban
\frac{dL(u,T_j,\tau)}{L(u,T_j,\tau)}=\gamma(u,T_j,\tau)dW^{Q^{T_i}}_u - \sum_{k=j+1}^{i-1}\frac{\tau L(\textcolor{red}{t},T_k,\tau) \gamma(u,T_k,\tau) \gamma(u,T_j,\tau) }{1+\tau L(\textcolor{red}{t},T_k,\tau)}du  
\ean

under  $Q^{T_i}$ for  $i\leq j$ and  $u \in [t \; T_s]$

\ban
\frac{dL(u,T_j,\tau)}{L(u,T_j,\tau)}=\gamma(u,T_j,\tau)dW^{Q^{T_i}}_u +\sum_{k=i}^{j}\frac{\tau L(\textcolor{red}{t},T_k,\tau)\gamma(u,T_k,\tau)\gamma(u,T_j,\tau)}{1+\tau L(\textcolor{red}{t},T_k,\tau)}dt
\ean


under this assumption the forward rates are lognormal


for $i>j+1$

\ban
L(T_s,T_j,\tau)&=&L(t,T_j,\tau)e^{\int_t^{T_s}\gamma(u,T_j,\tau)dW_u^{Q^{T_i}}-\frac{1}{2}\int_t^{T_s}\gamma(u,T_j,\tau)^2du}\\
& & e^{-\sum_{k=j+1}^{i-1}\frac{\tau L(t,T_k,\tau)}{1+\tau L(t,T_k,\tau)} \int_t^{T_s}\gamma(u,T_k,\tau) \gamma(u,T_j,\tau) du  }
\ean

for $j \geq i$

\ban
L(T_s,T_j,\tau)&=&L(t,T_j,\tau)e^{\int_t^{T_s}\gamma(u,T_j,\tau)dW_u^{Q^{T_i}}-\frac{1}{2}\int_t^{T_s}\gamma(u,T_j,\tau)^2du}\\
& & e^{+\sum_{k=i}^{j}\frac{\tau L(t,T_k,\tau)}{1+\tau L(t,T_k,\tau)}\int_t^{T_s} \gamma(u,T_k,\tau) \gamma(u,T_j,\tau) du  }
\ean

\newpage
we can write 

\ban
L(T_s,T_j,\tau)&=&L(t,T_j,\tau)e^{\int_t^{T_s}\gamma(u,T_j,\tau)dW_u^{Q^{T_i}}-\frac{1}{2}\int_t^{T_s}\gamma(u,T_j,\tau)^2du}\\
 &+& e^{\sum_{k=1}^{i-1}\frac{\tau L(t,T_k,\tau)}{1+\tau L(t,T_k,\tau)}\int_t^{T_s} \gamma(u,T_k,\tau) \gamma(u,T_j,\tau) du}
e^{- \sum_{k=1}^{j}\frac{\tau L(t,T_k,\tau)}{1+\tau L(t,T_k,\tau)}\int_t^{T_s} \gamma(u,T_k,\tau) \gamma(u,T_j,\tau) du  }
\ean




\ban
\xi_j^i&=&\int_t^{T_s}\gamma(u,T_j,\tau)dW_u^{Q^{T_i}}\\
\nu_{kj}&=&\int_t^{T_s} \gamma(u,T_k,\tau) \gamma(u,T_j,\tau) du \\
\beta_j^i&=&\sum_{k=1}^{i}\frac{\tau L(t,T_k,\tau)}{1+\tau L(t,T_k,\tau)}\int_t^{T_s} \gamma(u,T_k,\tau) \gamma(u,T_j,\tau) du\ean


\ban
L(T_s,T_j,\tau)&=&L(t,T_j,\tau)e^{\xi_j^i  -\frac{1}{2}\nu_{jj} + \beta_j^{i-1}-\beta_j^j  }
\ean



$\nu=(\nu_{kj})$ is variance covariance of the rates.

{\bf Rank one approximation}

There is a vector $\alpha=(\alpha_{s+1},\alpha_{s+2},..,\alpha_{M})^t$ with $\alpha_j\geq 0$ such that $\nu\sim\alpha \alpha^t $

then
 

\ban
\xi_j^i& \sim & \alpha_{j}X  \quad \textrm{with}  \quad X \quad {\cal N}(0,1)\\
\nu_{kj}& \sim & \alpha_{k}\alpha_{j} \\
\beta_j^i& \sim &\alpha_{j} \sum_{k=1}^{i}\frac{\tau L(t,T_k,\tau)}{1+\tau L(t,T_k,\tau)}\alpha_{k}\\
& \sim &\alpha_{j}d^i
\ean


\ban
L(T_s,T_j,\tau)&=&L(t,T_j,\tau)e^{\alpha_{j}X -\frac{1}{2}\alpha_{jj} + \alpha_j(d^{i-1}-d^j) }
\ean


\ban
&&E^{Q^{T_i}}_t\left[L(T_s,T_{i-1},\tau){\bf 1}_{D}\right]=\\
&&E^{Q^{T_i}}_t\left[L(t,T_{i-1},\tau)e^{ \alpha_{i-1}X -\frac{1}{2}\alpha_{i-1}\alpha_{i-1} } {\bf 1}_{\left( 1>\sum_{j=1}^Mc_j\prod_{k=0}^{j-1}\frac{1}{1+\tau L(t,T_k,\tau)} e^{\alpha_{k}X -\frac{1}{2}\alpha_{k}\alpha_k + \alpha_{k}(d^{i-1}-d^k)} \right)    }\right]
\ean

we note 

\ban
\phi_{i-1}(x)=\sum_{j=1}^Mc_j\prod_{k=0}^{j-1}\frac{1}{1+\tau L(t,T_k,\tau)} e^{\alpha_{k}x -\frac{1}{2}\alpha_{kk} + \alpha_{k}(d^{i-1}-d^k)}
\ean

recall that  $c_k\geq 0$ and $c_M > 1$ 

\ban
\lim_{x \rightarrow -\infty}\phi_{i-1}(x)&=&0\\
\lim_{x \rightarrow +\infty}\phi_{i-1}(x)&=&+\infty\\
\phi_{i-1}'(x)&>&0 
\ean  

so there is a unique $\bar x_{i-1}$ such that $\phi_{i-1}(\bar x_{i-1})=1$, finally the expectation is given by  

\ban
E^{Q^{T_i}}_t\left[L(T,T_{i-1},\tau){\bf 1}_{D}\right]=\int_{\bar x_{i-1}}^{+ \infty} L(t,T_{i-1},\tau)e^{\alpha_{i-1}x -\frac{1}{2}\alpha_{i-1}\alpha_{i-1}} \frac{1}{\sqrt {2\pi}}e^{-\frac{x^2}{2}}dx
\ean

and we have $\bar x_{i}=\bar x_{i-1}+d^{i-1}-d^{i}$

It is possible to use a rank k approximation, see Brace \cite{brace1}.


\paragraph{ The spot measure}

In  the HJM framework, where interest rates are continuously coumpounded,  one usually uses the cash as risk free asset which follows the dynamic

\ban
dB(t)=B(t)r(t)dt
\ean

In the LMM framework we deal with simple interest rates as such it is possible to define the discret tenor bank account noted $B_d(t)$ as follow:


$\eta(t)$ such that  $\eta(t)=n $ if $t \in [T_{n-1} \; T_{n}[$

\ban
B_d(0)&=&1\\
B_d(t)&=&\prod_{j=0}^{\eta(t)}(1+\tau L(T_j,T_j,\tau))B(t,T_{\eta(t)})
\ean

which is an asset with unit value at time $t=0$ and discretly compounded in the spot rates

using $B_d(t)$ as numeraire we can define the ``spot libor measure'' $Q^d$ under which  $L(t,T_i,\tau)$ follows the dynamic

\ban
\frac{dL(t,T_i,\tau)}{L(t,T_i,\tau)}= \sum_{k=\eta(t)}^{i}\frac{\tau L(t,T_k,\tau)\gamma(t,T_k,\tau)\gamma(t,T_i,\tau)}{1+\tau L(t,T_k,\tau)}dt + \gamma(t,T_i,\tau)dW^{Q^d}_t
\ean


\paragraph{ Pricing under $Q^d$}: the value at time $t=0$ of a security paying $\xi$ at $T_n$ is given by

\ban
\pi(0)=E^{Q^d}\left[ \frac{B^d(0)}{B^d(T_n)}\xi \right]
\ean

Remark: suppose $\xi=1$ then $\pi(0)=B(0,T_n)$

\ban
B(0,T_n)=E^{Q^d}\left[ \prod_{i=0}^{n-1}\frac{1}{(1+\tau L(T_i,T_i,\tau))} \right]
\ean

one should recover bond values from the forwards.
